theories/progLog.v
@@ -2,31 +2,10 @@ From iris.proofmode Require Import proofmode.
 From iris.base_logic Require Export invariants gen_heap.
 From iris.program_logic Require Export weakestpre ectx_lifting.
 From iris.algebra Require Import frac auth gmap excl.
+From Coq.Lists Require Import List.
 
 Section wp'.
   Context {Λ : language} `{!irisGS_gen hlc Λ Σ}.
-
-  Lemma wp_lift_atomic_step_fupd {s E1 E2 Φ} e1 :
-  to_val e1 = None →
-  (∀ σ1 ns κ κs nt, state_interp σ1 ns (κ ++ κs) nt ={E1}=∗
-    ⌜if s is NotStuck then reducible e1 σ1 else True⌝ ∗
-    ∀ e2 σ2 efs, ⌜prim_step e1 σ1 κ e2 σ2 efs⌝ -∗ £ 1 ={E1}[E2]▷=∗
-      state_interp σ2 (S ns) κs (length efs + nt) ∗
-      from_option Φ False (to_val e2) ∗
-      [∗ list] ef ∈ efs, WP ef @ s; ⊤ {{ fork_post }})
-  ⊢ WP e1 @ s; E1 {{ Φ }}.
-Proof.
-  iIntros (?) "H".
-  iApply (wp_lift_step_fupd s E1 _ e1)=>//; iIntros (σ1 ns κ κs nt) "Hσ1".
-  iMod ("H" $! σ1 with "Hσ1") as "[$ H]".
-  iApply fupd_mask_intro; first set_solver.
-  iIntros "Hclose" (e2 σ2 efs ?) "Hcred". iMod "Hclose" as "_".
-  iMod ("H" $! e2 σ2 efs with "[#] Hcred") as "H"; [done|].
-  iApply fupd_mask_intro; first set_solver. iIntros "Hclose !>".
-  iMod "Hclose" as "_". iMod "H" as "($ & HQ & $)".
-  destruct (to_val e2) eqn:?; last by iExFalso.
-  iApply wp_value; last done. by apply of_to_val.
-Qed.
 
   Lemma wp_lift_atomic_step_no_fork_fupd {s E1 E2 Φ} e1 :
     to_val e1 = None →
@@ -390,11 +369,11 @@ Notation "a ↦ₐ w" := (mapsto (L:=Addr) (V:=Word) a (DfracOwn 1) w) (at level
   Lemma wp_halt pc prog ll E :
     prog pc = Halt ->
     {{{ program_frag Program_name prog ∗ pc_frag PC_name pc ∗ tr_frag trace_name ll }}}
-      NextI @ E
+      (Instr Executable) @ E
     {{{ RET HaltedV; program_frag Program_name prog ∗ pc_frag PC_name pc ∗ tr_frag trace_name (NoLeak :: ll) }}}.
   Proof.
     iIntros (prpcHalt Φ) "(Hprog & Hpc & Hll) HΦ".
-    iApply wp_lift_atomic_step_fupd; auto.
+    iApply wp_lift_atomic_step_no_fork_fupd; auto.
     iIntros (σ ns κ κs nt) "(Hauthreg & Hauthmem & Hauthtrace & Hauthpc & Hauthprog)".
     destruct σ as [s ll'].
     simpl.
@@ -406,13 +385,392 @@ Notation "a ↦ₐ w" := (mapsto (L:=Addr) (V:=Word) a (DfracOwn 1) w) (at level
     - iPureIntro. apply normal_always_reducible.
     - iIntros (e2 σ2 efs) "%steps test".
       inversion steps; subst; simpl in *.
+      inversion H; subst.
+      simpl in *.
       rewrite prpcHalt in steps. rewrite prpcHalt. simpl in *. iFrame.
       iPoseProof (trace_update trace_name _ (NoLeak :: ll) with "[$Hauthtrace $Hll]") as "H".
       iMod "H". iModIntro. iNext. iModIntro.
       iDestruct "H" as "[Hauthll Hfragll]". iFrame.
-      iSplitR "test".
+      iSplitR.
+      + iPureIntro. reflexivity.
       + iApply "HΦ". iFrame.
-      + 
+  Qed.
+
+  Fixpoint regs_from_inputs {n : nat} (inputs : vec (Word + Register) n) : gset Register :=
+    match inputs with
+    | [# ] => ∅
+    | wr ::: inputs' => match wr with
+                        | inl _ => regs_from_inputs inputs'
+                        | inr r => {[ r ]} ∪ regs_from_inputs inputs'
+                        end
+    end.
+
+  Fixpoint replace_in_inputs {n : nat} (words : list Word) (inputs : vec (Word + Register) n)
+    : vec Word n :=
+    match inputs, words with
+    | Vector.nil, _ => Vector.nil
+    | Vector.cons input inputs', [] => match input with
+                                | inl word => Vector.cons word (replace_in_inputs words inputs')
+                                | inr _ => Vector.cons 0 (replace_in_inputs words inputs')
+                                end
+    | Vector.cons input inputs', word' :: words' => match input with
+                                | inl word => Vector.cons word (replace_in_inputs words inputs')
+                                | inr _ => Vector.cons word' (replace_in_inputs words' inputs')
+                                end
+    end.
+
+  Definition regs_of_argument (arg: Word + Register) : gset Register :=
+  match arg with
+  | inl _ => ∅
+  | inr r => {[ r ]}
+  end.
+
+Definition regs_of (i: instr): gset Register :=
+match i with
+    | Computation inputs rres f_result => {[ rres ]} ∪ regs_from_inputs inputs
+    | ControlFlow inputs dst f_condition => regs_of_argument dst ∪ regs_from_inputs inputs
+    | Load rres rsrc => {[ rres; rsrc ]}
+    | Store rdst src => {[ rdst ]} ∪ regs_of_argument src
+    | _ => ∅
+end.
+
+Lemma indom_regs_incl D (regs regs': Reg) :
+  D ⊆ dom regs →
+  regs ⊆ regs' →
+  ∀ r, r ∈ D →
+       ∃ (w:Word), (regs !! r = Some w) ∧ (regs' !! r = Some w).
+Proof.
+  intros * HD Hincl rr Hr.
+  assert (is_Some (regs !! rr)) as [w Hw].
+  { eapply @elem_of_dom with (D := gset Register). typeclasses eauto.
+    eapply elem_of_subseteq; eauto. }
+  exists w. split; auto. eapply lookup_weaken; eauto.
+Qed.
+
+Lemma indom_regs_incl_default D (regs regs': Reg) :
+  D ⊆ dom regs →
+  regs ⊆ regs' →
+  ∀ r, r ∈ D →
+       ∃ (w:Word), (regs !!! r = w) ∧ (regs' !!! r = w).
+Proof.
+  intros * HD Hincl rr Hr.
+  specialize (indom_regs_incl _ _ _ HD Hincl rr Hr) as [w [Hw Hw']].
+  unfold "!!!". unfold map_lookup_total. unfold default. simpl. rewrite Hw.
+  exists w. split; auto. rewrite (lookup_weaken _ _ _ _ Hw Hincl). reflexivity.
+Qed.
+
+Lemma gen_heap_update_inSepM :
+    ∀ {L V : Type} {EqDecision0 : EqDecision L}
+      {H : Countable L} {Σ : gFunctors}
+      {gen_heapG0 : gen_heapGS L V Σ}
+      (σ σ' : gmap L V) (l : L) (v : V),
+      is_Some (σ' !! l) →
+      gen_heap_interp σ
+      -∗ ([∗ map] k↦y ∈ σ', mapsto k (DfracOwn 1) y)
+      ==∗ gen_heap_interp (<[l:=v]> σ)
+          ∗ [∗ map] k↦y ∈ (<[l:=v]> σ'), mapsto k (DfracOwn 1) y.
+  Proof.
+    intros * Hσ'. destruct Hσ'.
+    rewrite (big_sepM_delete _ σ' l) //. iIntros "Hh [Hl Hmap]".
+    iMod (gen_heap_update with "Hh Hl") as "[Hh Hl]". iModIntro.
+    iSplitL "Hh"; eauto.
+    rewrite (big_sepM_delete _ (<[l:=v]> σ') l).
+    { rewrite delete_insert_delete. iFrame. }
+    rewrite lookup_insert //.
+  Qed.
+
+  Lemma gen_heap_valid_inSepM':
+    ∀ (L V : Type) (EqDecision0 : EqDecision L) (H : Countable L)
+      (Σ : gFunctors) (gen_heapG0 : gen_heapGS L V Σ)
+      (σ σ' : gmap L V) (q : Qp),
+      gen_heap_interp σ -∗
+      ([∗ map] k↦y ∈ σ', mapsto k (DfracOwn q) y) -∗
+      ⌜forall (l: L) (v: V), σ' !! l = Some v → σ !! l = Some v⌝.
+  Proof.
+    intros *. iIntros "? Hmap" (l v Hσ').
+    rewrite (big_sepM_delete _ σ' l) //. iDestruct "Hmap" as "[? ?]".
+    iApply (gen_heap_valid with "[$]"). eauto.
+  Qed.
+
+  Lemma gen_heap_valid_inclSepM:
+    ∀ (L V : Type) (EqDecision0 : EqDecision L) (H : Countable L)
+      (Σ : gFunctors) (gen_heapG0 : gen_heapGS L V Σ)
+      (σ σ' : gmap L V) (q : Qp),
+      gen_heap_interp σ -∗
+      ([∗ map] k↦y ∈ σ', mapsto k (DfracOwn q) y) -∗
+      ⌜σ' ⊆ σ⌝.
+  Proof.
+    intros *. iIntros "Hσ Hmap".
+    iDestruct (gen_heap_valid_inSepM' with "Hσ Hmap") as "#H".
+    iDestruct "H" as %Hincl. iPureIntro. intro l.
+    unfold option_relation.
+    destruct (σ' !! l) eqn:HH'; destruct (σ !! l) eqn:HH; naive_solver.
+  Qed.
+
+Lemma inputs_are_enough {B : Type} {n : nat} regs regs' (f_result : vec Word n -> B) (inputs : vec (Word + Register) n)
+  (inputs_in_regs : regs_from_inputs inputs ⊆ dom regs)
+  (regs_in_regs' : regs ⊆ regs') :
+  f_result (inputs_from_inputnatregs regs inputs) = f_result (inputs_from_inputnatregs regs' inputs).
+Proof.
+  induction inputs.
+  - reflexivity.
+  - destruct h.
+    + simpl. unfold regs_from_inputs in inputs_in_regs. simpl in inputs_in_regs.
+      apply (IHinputs (fun inputs' => f_result (w ::: inputs'))) in inputs_in_regs.
+      apply inputs_in_regs.
+    + simpl. specialize (indom_regs_incl_default _ _ _ inputs_in_regs regs_in_regs' r) as Hri.
+      destruct Hri.
+      { set_solver+. }
+      destruct H as [Hregs Hregs']. rewrite Hregs Hregs'.
+      simpl in inputs_in_regs. apply union_subseteq in inputs_in_regs. 
+      apply (IHinputs (fun inputs' => f_result (x ::: inputs'))).
+      destruct inputs_in_regs as [_ ->]. reflexivity.
+Qed.
+
+Lemma regs_of_computation {n : nat} (inputs : vec (Word + Register) n)
+    (rres : Register) (f_result : vec Word n -> Word) i :
+    i = Computation inputs rres f_result ->
+    regs_of i = {[ rres ]} ∪ regs_from_inputs inputs.
+Proof.
+  intros. subst.
+  reflexivity.
+Qed.
+
+Inductive Computation_spec {n : nat} (i: instr) (regs : Reg) (regs' : Reg) : Prop :=
+  | Computation_spec_success vn (inputs : vec (Word + Register) n) f_result (rres : Register) :
+      inputs_from_inputnatregs regs inputs = vn ->
+      (<[ rres := f_result vn ]> regs) = regs' ->
+      i = Computation inputs rres f_result ->
+      Computation_spec i regs regs'.
+
+Lemma wp_computation {n : nat} pc prog ll E (inputs : vec (Word + Register) n) rres f_result regs :
+  prog pc = Computation inputs rres f_result ->
+  regs_of (Computation inputs rres f_result) ⊆ dom regs →
+  {{{ program_frag Program_name prog ∗ pc_frag PC_name pc ∗ tr_frag trace_name ll ∗
+      [∗ map] k↦y ∈ regs, k ↦ᵣ y }}}
+      (Instr Executable) @ E
+  {{{ regs', RET NextIV; program_frag Program_name prog ∗ pc_frag PC_name (pc + 1) ∗ tr_frag trace_name (NoLeak :: ll) ∗
+    ⌜ Computation_spec (n := n) (Computation inputs rres f_result) regs regs' ⌝ ∗
+    [∗ map] k↦y ∈ regs', k ↦ᵣ y
+     }}}.
+  Proof.
+    iIntros (prpcHalt regs_subset Φ) "(Hprog & Hpc & Hll & HlistOfRegs) HΦ".
+    iApply wp_lift_atomic_step_no_fork_fupd; auto.
+    iIntros (σ ns κ κs nt) "(Hreg & Hmem & Hauthtrace & Hauthpc & Hauthprog)".
+    destruct σ as [s ll'].
+    simpl.
+    iDestruct (@trace_full_frag_eq with "Hauthtrace Hll") as %?; subst; auto.
+    iDestruct (@pc_full_frag_eq with "Hauthpc Hpc") as %?; subst; auto.
+    iDestruct (@program_full_frag_eq with "Hauthprog Hprog") as %?; subst; auto.
+    iPoseProof (trace_update trace_name _ (NoLeak :: ll) with "[$Hauthtrace $Hll]") as "H1".
+    iPoseProof (pc_update PC_name _ (PC (s.2) + 1) with "[$Hauthpc $Hpc]") as "H2".
+    
+
+    iDestruct (gen_heap_valid_inclSepM with "Hreg HlistOfRegs") as %Hregs.
+    specialize (indom_regs_incl _ _ _ regs_subset Hregs) as Hri.
+    destruct (Hri rres) as [wdst [H'dst Hdst]]. by set_solver+.        
+    iMod "H1". iMod "H2". iModIntro.
+
+    iDestruct "H1" as "[Hauthll Hfragll]". iDestruct "H2" as "[Hauthpc Hfragpc]".
+    iSplitR.
+    - iPureIntro. apply normal_always_reducible.
+    - iIntros (e2 σ2 efs) "%steps _".
+      inversion steps; subst; simpl in *.
+      inversion H; subst.
+      simpl in *.
+      rewrite prpcHalt in steps. rewrite prpcHalt. simpl in *.     
+      iFrame.
+      unfold incr_PC. rewrite -(update_pc_no_change_reg).
+      rewrite reg_is_updated_value.
+      iMod ((gen_heap_update_inSepM _ _ rres) with "Hreg HlistOfRegs") as "[Hr Hmap]".
+      { eauto.  }
+      iModIntro. iNext. iModIntro.
+      iFrame.
+      iSplitR.
+      { iPureIntro. reflexivity. }
+      iApply "HΦ". iFrame.
+      iPureIntro.
+      econstructor; try reflexivity.
+      rewrite (inputs_are_enough regs (reg φ)); auto. apply union_subseteq in regs_subset as [_ ->]. reflexivity.
+Qed.
+
+Lemma regs_of_control_flow {n : nat} (inputs : vec (Word + Register) n)
+    (dst : Word + Register) (f_condition : vec Word n -> bool) i :
+    i = ControlFlow inputs dst f_condition ->
+    regs_of i = regs_of_argument dst ∪ regs_from_inputs inputs.
+Proof.
+  intros. subst.
+  reflexivity.
+Qed.
+
+Inductive Control_flow_spec {n : nat} (i : instr) (pc pc' : Word) : Prop :=
+  | Control_flow_spec_true_success vn (inputs : vec (Word + Register) n) (regs : Reg) f_condition (dst : Word + Register) :
+      inputs_from_inputnatregs regs inputs = vn ->
+      f_condition vn = true ->
+      wordreg_to_word regs dst = pc' ->
+      i = ControlFlow inputs dst f_condition ->
+      Control_flow_spec i pc pc'
+  | Control_flow_spec_false_success vn (inputs : vec (Word + Register) n) (regs : Reg) f_condition (dst : Word + Register) :
+      inputs_from_inputnatregs regs inputs = vn ->
+      f_condition vn = false ->
+      pc + 1 = pc' ->
+      i = ControlFlow inputs dst f_condition ->
+      Control_flow_spec i pc pc'.
+
+Lemma wp_control_flow {n : nat} pc prog ll E (inputs : vec (Word + Register) n) dst f_condition regs :
+  prog pc = ControlFlow inputs dst f_condition ->
+  regs_of (ControlFlow inputs dst f_condition) ⊆ dom regs →
+  {{{ program_frag Program_name prog ∗ pc_frag PC_name pc ∗ tr_frag trace_name ll ∗
+      [∗ map] k↦y ∈ regs, k ↦ᵣ y }}}
+      (Instr Executable) @ E
+  {{{ pc', RET NextIV; program_frag Program_name prog ∗ pc_frag PC_name pc' ∗ tr_frag trace_name (ControlFlowLeak (f_condition (inputs_from_inputnatregs (regs) inputs)) :: ll) ∗
+    ⌜ Control_flow_spec (n := n) (ControlFlow inputs dst f_condition) pc pc' ⌝ ∗
+    [∗ map] k↦y ∈ regs, k ↦ᵣ y
+     }}}.
+  Proof.
+    iIntros (prpcHalt regs_subset Φ) "(Hprog & Hpc & Hll & HlistOfRegs) HΦ".
+    iApply wp_lift_atomic_step_no_fork_fupd; auto.
+    iIntros (σ ns κ κs nt) "(Hreg & Hmem & Hauthtrace & Hauthpc & Hauthprog)".
+    destruct σ as [s ll'].
+    simpl.
+    iDestruct (@trace_full_frag_eq with "Hauthtrace Hll") as %?; subst; auto.
+    iDestruct (@pc_full_frag_eq with "Hauthpc Hpc") as %?; subst; auto.
+    iDestruct (@program_full_frag_eq with "Hauthprog Hprog") as %?; subst; auto.
+    iDestruct (gen_heap_valid_inclSepM with "Hreg HlistOfRegs") as %Hregs.   
+    iModIntro.
+    iSplitR.
+    - iPureIntro. apply normal_always_reducible.
+    - iIntros (e2 σ2 efs) "%steps _".
+      inversion steps; subst; simpl in *.
+      inversion H; subst.
+      simpl in *.
+      rewrite prpcHalt in steps. rewrite prpcHalt. simpl in *.
+      destruct (f_condition (inputs_from_inputnatregs (reg φ) inputs)) as [|] eqn:Hcondition.
+      all: iPoseProof (trace_update trace_name _ (ControlFlowLeak (f_condition (inputs_from_inputnatregs (reg φ) inputs)) :: ll) with "[$Hauthtrace $Hll]") as "H1".
+      1: iPoseProof (pc_update PC_name _ (wordreg_to_word (reg φ) dst) with "[$Hauthpc $Hpc]") as "H2".
+      2: iPoseProof (pc_update PC_name _ (PC φ + 1) with "[$Hauthpc $Hpc]") as "H2".
+      all: iMod "H1"; iMod "H2"; iDestruct "H1" as "[Hauthll Hfragll]"; iDestruct "H2" as "[Hauthpc Hfragpc]";
+      rewrite Hcondition; iFrame.
+      all: iModIntro; iNext; iModIntro.
+      all: iSplitR; try (iPureIntro; reflexivity).
+      all: iApply "HΦ".
+      all: assert ((f_condition (inputs_from_inputnatregs regs inputs) = f_condition (inputs_from_inputnatregs (reg φ) inputs))) as Hreg_regφ;
+      try (apply (inputs_are_enough regs (reg φ)); auto; apply union_subseteq in regs_subset as [_ ->]; reflexivity); rewrite Hreg_regφ Hcondition.
+      all: iFrame.
+      all: iPureIntro.
+      + eapply Control_flow_spec_true_success; eauto.
+      + eapply Control_flow_spec_false_success; eauto.
+Qed.
+
+Lemma wp_load {n : nat} pc prog ll E rres rsrc regs v :
+  prog pc = Load rres rsrc ->
+  regs_of (Load rres rsrc) ⊆ dom regs →
+  {{{ program_frag Program_name prog ∗ pc_frag PC_name pc ∗ tr_frag trace_name ll ∗
+      ([∗ map] k↦y ∈ regs, k ↦ᵣ y) ∗
+      word_to_addr (regs !!! rsrc) ↦ₐ v }}}
+      (Instr Executable) @ E
+  {{{ RET NextIV; program_frag Program_name prog ∗ pc_frag PC_name (pc + 1) ∗
+      tr_frag trace_name (LoadLeak (regs !!! rsrc) :: ll) ∗
+      [∗ map] k↦y ∈ <[ rres := v ]>regs, k ↦ᵣ y
+     }}}.
+  Proof.
+    iIntros (prpcHalt regs_subset Φ) "(Hprog & Hpc & Hll & HlistOfRegs & Haddrv) HΦ".
+    iApply wp_lift_atomic_step_no_fork_fupd; auto.
+    iIntros (σ ns κ κs nt) "(Hreg & Hmem & Hauthtrace & Hauthpc & Hauthprog)".
+    destruct σ as [s ll'].
+    simpl.
+    iDestruct (@trace_full_frag_eq with "Hauthtrace Hll") as %?; subst; auto.
+    iDestruct (@pc_full_frag_eq with "Hauthpc Hpc") as %?; subst; auto.
+    iDestruct (@program_full_frag_eq with "Hauthprog Hprog") as %?; subst; auto.
+    iDestruct (gen_heap_valid_inclSepM with "Hreg HlistOfRegs") as %Hregs.
+    iModIntro.
+
+    iSplitR.
+    { iPureIntro. apply normal_always_reducible. }
+    iIntros (e2 σ2 efs) "%steps _".
+    inversion steps; subst; simpl in *.
+    inversion H; subst.
+    simpl in *.
+    rewrite prpcHalt in steps. rewrite prpcHalt. simpl in *.
+
+    iPoseProof (trace_update trace_name _ (LoadLeak (reg φ !!! rsrc) :: ll) with "[$Hauthtrace $Hll]") as "H1".
+    iPoseProof (pc_update PC_name _ (PC φ + 1) with "[$Hauthpc $Hpc]") as "H2".
+    iMod "H1"; iMod "H2"; iDestruct "H1" as "[Hauthll Hfragll]"; iDestruct "H2" as "[Hauthpc Hfragpc]".
+    
+    unfold incr_PC. rewrite -update_pc_no_change_reg. rewrite reg_is_updated_value.
+    iMod ((gen_heap_update_inSepM _ _ rres) with "Hreg HlistOfRegs") as "[Hr Hmap]".
+    { eapply @elem_of_dom with (D := gset Register). typeclasses eauto.
+    eapply elem_of_subseteq; eauto. set_solver. }
+    iPoseProof (gen_heap_valid with "Hmem Haddrv") as "%Hmem'".
+    iModIntro. iNext. iModIntro. iFrame.
+    iSplitR.
+    { iPureIntro. reflexivity. }
+    
+    iApply "HΦ"; iFrame.
+    specialize (indom_regs_incl_default _ _ _ regs_subset Hregs rsrc) as Hri.
+    destruct Hri as [w [Hw Hw']]. { set_solver. }
+    rewrite Hw. rewrite Hw'. iFrame.
+    rewrite Hw in Hmem'. unfold word_to_addr in Hmem'.
+    assert (mem φ !!! w = v) as Hmem''. { unfold "!!!". unfold map_lookup_total. unfold default. rewrite Hmem'. reflexivity. }
+    rewrite Hmem''. iFrame.
+Qed.
+
+Lemma wp_store {n : nat} pc prog ll E rdst src regs v :
+  prog pc = Store rdst src ->
+  regs_of (Store rdst src) ⊆ dom regs →
+  {{{ program_frag Program_name prog ∗ pc_frag PC_name pc ∗ tr_frag trace_name ll ∗
+      ([∗ map] k↦y ∈ regs, k ↦ᵣ y) ∗
+      word_to_addr (regs !!! rdst) ↦ₐ v }}}
+      (Instr Executable) @ E
+  {{{ RET NextIV; program_frag Program_name prog ∗ pc_frag PC_name (pc + 1) ∗
+      tr_frag trace_name (StoreLeak (wordreg_to_word regs src) :: ll) ∗
+      ([∗ map] k↦y ∈ regs, k ↦ᵣ y) ∗
+      word_to_addr (regs !!! rdst) ↦ₐ wordreg_to_word regs src
+     }}}.
+  Proof.
+    iIntros (prpcHalt regs_subset Φ) "(Hprog & Hpc & Hll & HlistOfRegs & Haddrv) HΦ".
+    iApply wp_lift_atomic_step_no_fork_fupd; auto.
+    iIntros (σ ns κ κs nt) "(Hreg & Hmem & Hauthtrace & Hauthpc & Hauthprog)".
+    destruct σ as [s ll'].
+    simpl.
+    iDestruct (@trace_full_frag_eq with "Hauthtrace Hll") as %?; subst; auto.
+    iDestruct (@pc_full_frag_eq with "Hauthpc Hpc") as %?; subst; auto.
+    iDestruct (@program_full_frag_eq with "Hauthprog Hprog") as %?; subst; auto.
+    iDestruct (gen_heap_valid_inclSepM with "Hreg HlistOfRegs") as %Hregs.
+    iModIntro.
+
+    iSplitR.
+    { iPureIntro. apply normal_always_reducible. }
+    iIntros (e2 σ2 efs) "%steps _".
+    inversion steps; subst; simpl in *.
+    inversion H; subst.
+    simpl in *.
+    rewrite prpcHalt in steps. rewrite prpcHalt. simpl in *.
+
+    iPoseProof (trace_update trace_name _ (StoreLeak (wordreg_to_word regs src) :: ll) with "[$Hauthtrace $Hll]") as "H1".
+    iPoseProof (pc_update PC_name _ (PC φ + 1) with "[$Hauthpc $Hpc]") as "H2".
+    iMod "H1"; iMod "H2"; iDestruct "H1" as "[Hauthll Hfragll]"; iDestruct "H2" as "[Hauthpc Hfragpc]".
+    
+    unfold incr_PC. rewrite -update_pc_no_change_reg. rewrite -update_mem_no_change_reg.
+    iPoseProof (gen_heap_valid with "Hmem Haddrv") as "%Hmem'".
+    
+    iMod ((gen_heap_update _ (regs !!! rdst)) with "Hmem Haddrv") as "[Hr Hmap]".
+    specialize (indom_regs_incl_default _ _ _ regs_subset Hregs rdst) as Hri.
+    destruct Hri as [w [Hw Hw']]. { set_solver. }
+    rewrite Hw Hw'.
+
+    iModIntro. iNext. iModIntro. iFrame.
+    iSplitR.
+    { iPureIntro. reflexivity. }
+    
+    iSplitL "Hauthll".
+    all: destruct src; simpl; iFrame.
+    all: try iApply "HΦ"; iFrame.
+    all: specialize (indom_regs_incl_default _ _ _ regs_subset Hregs r) as Hri.
+    all: destruct Hri as [w1 [Hw1 Hw1']]; try set_solver; rewrite Hw1 Hw1'; iFrame.
+Qed.
 
 
-  End asm_lang_rules.
+
+
+End asm_lang_rules.
